### Сложение матриц
#### Пример
$
\color{red}{A} = \begin{pmatrix}
\color{red}{1} & \color{red}{4} & \color{red}{-5} \\\\ 
\color{red}{-11} & \color{red}{7} & \color{red}{3}
\end{pmatrix};
\color{green}{B} = \begin{pmatrix}
\color{green}{4} & \color{green}{8} & \color{green}{1} \\\\ 
\color{green}{2} & \color{green}{-10} & \color{green}{3}
\end{pmatrix};
$
$
\color{blue}{C}=\color{red}{A}+\color{green}{B}.
$
$
\begin{pmatrix}
\color{red}{1} & \color{red}{4} & \color{red}{-5} \\\\ 
\color{red}{-11} & \color{red}{7} & \color{red}{3}
\end{pmatrix} +
\begin{pmatrix}
\color{green}{4} & \color{green}{8} & \color{green}{1} \\\\ 
\color{green}{2} & \color{green}{-10} & \color{green}{3}
\end{pmatrix} =
$
$
= \begin{pmatrix}
\color{red}{1}+\color{green}{4} & \color{red}{4}+\color{green}{8} & \color{red}{-5}+\color{green}{1} \\\\ 
\color{red}{-11}+\color{green}{2} & \color{red}{7}+\color{green}{(-10)} & \color{red}{3}+\color{green}{3}
\end{pmatrix}=
$
$
= \begin{pmatrix}
\color{blue}{5} & \color{blue}{12} & \color{blue}{-4} \\\\ 
\color{blue}{-9} & \color{blue}{-3} & \color{blue}{6}
\end{pmatrix}= \color{blue}{C}
$